powerpc/SelectOp.v
@@ -60,14 +60,9 @@ Definition addrstack (ofs: int) :=
 
 (** ** Integer logical negation *)
 
-(** The natural way to write smart constructors is by pattern-matching
-  on their arguments, recognizing cases where cheaper operators
-  or combined operators are applicable.  For instance, integer logical
-  negation has three special cases (not-and, not-or and not-xor),
-  along with a default case that uses not-or over its arguments and itself.
-  This is written naively as follows:
+(** Original definition:
 <<
-Definition notint (e: expr) :=
+Nondetfunction notint (e: expr) :=
   match e with
   | Eop (Ointconst n) Enil => Eop (Ointconst (Int.not n)) Enil
   | Eop Oand (t1:::t2:::Enil) => Eop Onand (t1:::t2:::Enil)
@@ -76,80 +71,38 @@ Definition notint (e: expr) :=
   | _ => Elet e (Eop Onor (Eletvar O ::: Eletvar O ::: Enil))
   end.
 >>
-  However, Coq expands complex pattern-matchings like the above into
-  elementary matchings over all constructors of an inductive type,
-  resulting in much duplication of the final catch-all case.
-  Such duplications generate huge executable code and duplicate
-  cases in the correctness proofs.
-
-  To limit this duplication, we use the following trick due to
-  Yves Bertot.  We first define a dependent inductive type that
-  characterizes the expressions that match each of the 4 cases of interest.
 *)
 
 Inductive notint_cases: forall (e: expr), Type :=
-  | notint_case1:
-      forall n,
-      notint_cases (Eop (Ointconst n) Enil)
-  | notint_case2:
-      forall t1 t2,
-      notint_cases (Eop Oand (t1:::t2:::Enil))
-  | notint_case3:
-      forall t1 t2,
-      notint_cases (Eop Oor (t1:::t2:::Enil))
-  | notint_case4:
-      forall t1 t2,
-      notint_cases (Eop Oxor (t1:::t2:::Enil))
-  | notint_default:
-      forall (e: expr),
-      notint_cases e.
-
-(** We then define a classification function that takes an expression
-  and return the case in which it falls.  Note that the catch-all case
-  [notint_default] does not state that it is mutually exclusive with
-  the first three, more specific cases.  The classification function
-  nonetheless chooses the specific cases in preference to the catch-all
-  case. *)
+  | notint_case1: forall n, notint_cases (Eop (Ointconst n) Enil)
+  | notint_case2: forall t1 t2, notint_cases (Eop Oand (t1:::t2:::Enil))
+  | notint_case3: forall t1 t2, notint_cases (Eop Oor (t1:::t2:::Enil))
+  | notint_case4: forall t1 t2, notint_cases (Eop Oxor (t1:::t2:::Enil))
+  | notint_default: forall (e: expr), notint_cases e.
 
 Definition notint_match (e: expr) :=
-  match e as z1 return notint_cases z1 with
-  | Eop (Ointconst n) Enil =>
-      notint_case1 n
-  | Eop Oand (t1:::t2:::Enil) =>
-      notint_case2 t1 t2
-  | Eop Oor (t1:::t2:::Enil) =>
-      notint_case3 t1 t2
-  | Eop Oxor (t1:::t2:::Enil) =>
-      notint_case4 t1 t2
-  | e =>
-      notint_default e
+  match e as zz1 return notint_cases zz1 with
+  | Eop (Ointconst n) Enil => notint_case1 n
+  | Eop Oand (t1:::t2:::Enil) => notint_case2 t1 t2
+  | Eop Oor (t1:::t2:::Enil) => notint_case3 t1 t2
+  | Eop Oxor (t1:::t2:::Enil) => notint_case4 t1 t2
+  | e => notint_default e
   end.
-
-(** Finally, the [notint] function we need is defined by a 4-case match
-  over the result of the classification function.  Thus, no duplication
-  of the right-hand sides of this match occur, and the proof has only
-  4 cases to consider (it proceeds by case over [notint_match e]).
-  Since the default case is not obviously exclusive with the three
-  specific cases, it is important that its right-hand side is
-  semantically correct for all possible values of [e], which is the
-  case here and for all other smart constructors. *)
 
 Definition notint (e: expr) :=
   match notint_match e with
-  | notint_case1 n =>
+  | notint_case1 n => (* Eop (Ointconst n) Enil *) 
       Eop (Ointconst (Int.not n)) Enil
-  | notint_case2 t1 t2 =>
+  | notint_case2 t1 t2 => (* Eop Oand (t1:::t2:::Enil) *) 
       Eop Onand (t1:::t2:::Enil)
-  | notint_case3 t1 t2 =>
+  | notint_case3 t1 t2 => (* Eop Oor (t1:::t2:::Enil) *) 
       Eop Onor (t1:::t2:::Enil)
-  | notint_case4 t1 t2 =>
+  | notint_case4 t1 t2 => (* Eop Oxor (t1:::t2:::Enil) *) 
       Eop Onxor (t1:::t2:::Enil)
   | notint_default e =>
       Elet e (Eop Onor (Eletvar O ::: Eletvar O ::: Enil))
   end.
 
-(** This programming pattern will be applied systematically for the
-  other smart constructors in this file. *)
 
 (** ** Boolean negation *)
 
@@ -170,8 +123,9 @@ Fixpoint notbool (e: expr) {struct e} : expr :=
 
 (** ** Integer addition and pointer addition *)
 
-(*
-Definition addimm (n: int) (e: expr) :=
+(** Original definition:
+<<
+Nondetfunction addimm (n: int) (e: expr) :=
   if Int.eq n Int.zero then e else
   match e with
   | Eop (Ointconst m) Enil       => Eop (Ointconst(Int.add n m)) Enil
@@ -180,336 +134,200 @@ Definition addimm (n: int) (e: expr) :=
   | Eop (Oaddimm m) (t ::: Enil) => Eop (Oaddimm(Int.add n m)) (t ::: Enil)
   | _                            => Eop (Oaddimm n) (e ::: Enil)
   end.
+>>
 *)
 
-(** Addition of an integer constant. *)
-
 Inductive addimm_cases: forall (e: expr), Type :=
-  | addimm_case1:
-      forall (m: int),
-      addimm_cases (Eop (Ointconst m) Enil)
-  | addimm_case2:
-      forall (s: ident) (m: int),
-      addimm_cases (Eop (Oaddrsymbol s m) Enil)
-  | addimm_case3:
-      forall (m: int),
-      addimm_cases (Eop (Oaddrstack m) Enil)
-  | addimm_case4:
-      forall (m: int) (t: expr),
-      addimm_cases (Eop (Oaddimm m) (t ::: Enil))
-  | addimm_default:
-      forall (e: expr),
-      addimm_cases e.
+  | addimm_case1: forall m, addimm_cases (Eop (Ointconst m) Enil)
+  | addimm_case2: forall s m, addimm_cases (Eop (Oaddrsymbol s m) Enil)
+  | addimm_case3: forall m, addimm_cases (Eop (Oaddrstack m) Enil)
+  | addimm_case4: forall m t, addimm_cases (Eop (Oaddimm m) (t ::: Enil))
+  | addimm_default: forall (e: expr), addimm_cases e.
 
 Definition addimm_match (e: expr) :=
-  match e as z1 return addimm_cases z1 with
-  | Eop (Ointconst m) Enil =>
-      addimm_case1 m
-  | Eop (Oaddrsymbol s m) Enil =>
-      addimm_case2 s m
-  | Eop (Oaddrstack m) Enil =>
-      addimm_case3 m
-  | Eop (Oaddimm m) (t ::: Enil) =>
-      addimm_case4 m t
-  | e =>
-      addimm_default e
+  match e as zz1 return addimm_cases zz1 with
+  | Eop (Ointconst m) Enil => addimm_case1 m
+  | Eop (Oaddrsymbol s m) Enil => addimm_case2 s m
+  | Eop (Oaddrstack m) Enil => addimm_case3 m
+  | Eop (Oaddimm m) (t ::: Enil) => addimm_case4 m t
+  | e => addimm_default e
   end.
 
 Definition addimm (n: int) (e: expr) :=
-  if Int.eq n Int.zero then e else
-  match addimm_match e with
-  | addimm_case1 m =>
+ if Int.eq n Int.zero then e else match addimm_match e with
+  | addimm_case1 m => (* Eop (Ointconst m) Enil *) 
       Eop (Ointconst(Int.add n m)) Enil
-  | addimm_case2 s m =>
+  | addimm_case2 s m => (* Eop (Oaddrsymbol s m) Enil *) 
       Eop (Oaddrsymbol s (Int.add n m)) Enil
-  | addimm_case3 m =>
+  | addimm_case3 m => (* Eop (Oaddrstack m) Enil *) 
       Eop (Oaddrstack (Int.add n m)) Enil
-  | addimm_case4 m t =>
+  | addimm_case4 m t => (* Eop (Oaddimm m) (t ::: Enil) *) 
       Eop (Oaddimm(Int.add n m)) (t ::: Enil)
   | addimm_default e =>
       Eop (Oaddimm n) (e ::: Enil)
   end.
 
-(** Addition of two integer or pointer expressions. *)
 
-(*
-Definition add (e1: expr) (e2: expr) :=
+(** Original definition:
+<<
+Nondetfunction add (e1: expr) (e2: expr) :=
   match e1, e2 with
-  | Eop (Ointconst n1) Enil, t2 => addimm n1 t2
-  | Eop (Oaddimm n1) (t1:::Enil), Eop (Oaddimm n2) (t2:::Enil) => addimm (Int.add n1 n2) (Eop Oadd (t1:::t2:::Enil))
-  | Eop(Oaddimm n1) (t1:::Enil)), t2 => addimm n1 (Eop Oadd (t1:::t2:::Enil))
-  | t1, Eop (Ointconst n2) Enil => addimm n2 t1
-  | t1, Eop (Oaddimm n2) (t2:::Enil) => addimm n2 (Eop Oadd (t1:::t2:::Enil))
-  | Eop (Oaddrsymbol s n1) Enil, Eop (Oaddimm n2) (t2:::Enil) => Eop Oadd (Eop (Oaddrsymbol s (Int.add n1 n2)) Enil ::: t2 ::: Enil)
-  | Eop (Oaddrstack n1) Enil, Eop (Oaddimm n2) (t2:::Enil) => Eop Oadd (Eop (Oaddstack (Int.add n1 n2)) Enil ::: t2 ::: Enil)
-  | _, _ => Eop Oadd (e1:::e2:::Enil)
+  | Eop (Ointconst n1) Enil, t2 =>
+      addimm n1 t2
+  | Eop (Oaddimm n1) (t1:::Enil), Eop (Oaddimm n2) (t2:::Enil) =>
+      addimm (Int.add n1 n2) (Eop Oadd (t1:::t2:::Enil))
+  | Eop (Oaddimm n1) (t1:::Enil), t2 =>
+      addimm n1 (Eop Oadd (t1:::t2:::Enil))
+  | Eop (Oaddrsymbol s n1) Enil, Eop (Oaddimm n2) (t2:::Enil) =>
+      Eop Oadd (Eop (Oaddrsymbol s (Int.add n1 n2)) Enil ::: t2 ::: Enil)
+  | Eop (Oaddrstack n1) Enil, Eop (Oaddimm n2) (t2:::Enil) =>
+      Eop Oadd (Eop (Oaddrstack (Int.add n1 n2)) Enil ::: t2 ::: Enil)
+  | t1, Eop (Ointconst n2) Enil =>
+      addimm n2 t1
+  | t1, Eop (Oaddimm n2) (t2:::Enil) =>
+      addimm n2 (Eop Oadd (t1:::t2:::Enil))
+  | _, _ =>
+      Eop Oadd (e1:::e2:::Enil)
   end.
+>>
 *)
 
 Inductive add_cases: forall (e1: expr) (e2: expr), Type :=
-  | add_case1:
-      forall (n1: int) (t2: expr),
-      add_cases (Eop (Ointconst n1) Enil) (t2)
-  | add_case2:
-      forall (n1: int) (t1: expr) (n2: int) (t2: expr),
-      add_cases (Eop (Oaddimm n1) (t1:::Enil)) (Eop (Oaddimm n2) (t2:::Enil))
-  | add_case3:
-      forall (n1: int) (t1: expr) (t2: expr),
-      add_cases (Eop(Oaddimm n1) (t1:::Enil)) (t2)
-  | add_case4:
-      forall (t1: expr) (n2: int),
-      add_cases (t1) (Eop (Ointconst n2) Enil)
-  | add_case5:
-      forall (t1: expr) (n2: int) (t2: expr),
-      add_cases (t1) (Eop (Oaddimm n2) (t2:::Enil))
-  | add_case6:
-      forall s n1 n2 t2,
-      add_cases (Eop (Oaddrsymbol s n1) Enil) (Eop (Oaddimm n2) (t2:::Enil))
-  | add_case7:
-      forall n1 n2 t2,
-      add_cases (Eop (Oaddrstack n1) Enil) (Eop (Oaddimm n2) (t2:::Enil))
-  | add_default:
-      forall (e1: expr) (e2: expr),
-      add_cases e1 e2.
-
-Definition add_match_aux (e1: expr) (e2: expr) :=
-  match e2 as z2 return add_cases e1 z2 with
-  | Eop (Ointconst n2) Enil =>
-      add_case4 e1 n2
-  | Eop (Oaddimm n2) (t2:::Enil) =>
-      add_case5 e1 n2 t2
-  | e2 =>
-      add_default e1 e2
-  end.
+  | add_case1: forall n1 t2, add_cases (Eop (Ointconst n1) Enil) (t2)
+  | add_case2: forall n1 t1 n2 t2, add_cases (Eop (Oaddimm n1) (t1:::Enil)) (Eop (Oaddimm n2) (t2:::Enil))
+  | add_case3: forall n1 t1 t2, add_cases (Eop (Oaddimm n1) (t1:::Enil)) (t2)
+  | add_case4: forall s n1 n2 t2, add_cases (Eop (Oaddrsymbol s n1) Enil) (Eop (Oaddimm n2) (t2:::Enil))
+  | add_case5: forall n1 n2 t2, add_cases (Eop (Oaddrstack n1) Enil) (Eop (Oaddimm n2) (t2:::Enil))
+  | add_case6: forall t1 n2, add_cases (t1) (Eop (Ointconst n2) Enil)
+  | add_case7: forall t1 n2 t2, add_cases (t1) (Eop (Oaddimm n2) (t2:::Enil))
+  | add_default: forall (e1: expr) (e2: expr), add_cases e1 e2.
 
 Definition add_match (e1: expr) (e2: expr) :=
-  match e1 as z1, e2 as z2 return add_cases z1 z2 with
-  | Eop (Ointconst n1) Enil, t2 =>
-      add_case1 n1 t2
-  | Eop (Oaddimm n1) (t1:::Enil), Eop (Oaddimm n2) (t2:::Enil) =>
-      add_case2 n1 t1 n2 t2
-  | Eop(Oaddimm n1) (t1:::Enil), t2 =>
-      add_case3 n1 t1 t2
-  | Eop (Oaddrsymbol s n1) Enil, Eop (Oaddimm n2) (t2:::Enil) => 
-      add_case6 s n1 n2 t2
-  | Eop (Oaddrstack n1) Enil, Eop (Oaddimm n2) (t2:::Enil) =>
-      add_case7 n1 n2 t2
-  | e1, e2 =>
-      add_match_aux e1 e2
+  match e1 as zz1, e2 as zz2 return add_cases zz1 zz2 with
+  | Eop (Ointconst n1) Enil, t2 => add_case1 n1 t2
+  | Eop (Oaddimm n1) (t1:::Enil), Eop (Oaddimm n2) (t2:::Enil) => add_case2 n1 t1 n2 t2
+  | Eop (Oaddimm n1) (t1:::Enil), t2 => add_case3 n1 t1 t2
+  | Eop (Oaddrsymbol s n1) Enil, Eop (Oaddimm n2) (t2:::Enil) => add_case4 s n1 n2 t2
+  | Eop (Oaddrstack n1) Enil, Eop (Oaddimm n2) (t2:::Enil) => add_case5 n1 n2 t2
+  | t1, Eop (Ointconst n2) Enil => add_case6 t1 n2
+  | t1, Eop (Oaddimm n2) (t2:::Enil) => add_case7 t1 n2 t2
+  | e1, e2 => add_default e1 e2
   end.
 
 Definition add (e1: expr) (e2: expr) :=
   match add_match e1 e2 with
-  | add_case1 n1 t2 =>
+  | add_case1 n1 t2 => (* Eop (Ointconst n1) Enil, t2 *) 
       addimm n1 t2
-  | add_case2 n1 t1 n2 t2 =>
+  | add_case2 n1 t1 n2 t2 => (* Eop (Oaddimm n1) (t1:::Enil), Eop (Oaddimm n2) (t2:::Enil) *) 
       addimm (Int.add n1 n2) (Eop Oadd (t1:::t2:::Enil))
-  | add_case3 n1 t1 t2 =>
+  | add_case3 n1 t1 t2 => (* Eop (Oaddimm n1) (t1:::Enil), t2 *) 
       addimm n1 (Eop Oadd (t1:::t2:::Enil))
-  | add_case4 t1 n2 =>
-      addimm n2 t1
-  | add_case5 t1 n2 t2 =>
-      addimm n2 (Eop Oadd (t1:::t2:::Enil))
-  | add_case6 s n1 n2 t2 =>
+  | add_case4 s n1 n2 t2 => (* Eop (Oaddrsymbol s n1) Enil, Eop (Oaddimm n2) (t2:::Enil) *) 
       Eop Oadd (Eop (Oaddrsymbol s (Int.add n1 n2)) Enil ::: t2 ::: Enil)
-  | add_case7 n1 n2 t2 =>
+  | add_case5 n1 n2 t2 => (* Eop (Oaddrstack n1) Enil, Eop (Oaddimm n2) (t2:::Enil) *) 
       Eop Oadd (Eop (Oaddrstack (Int.add n1 n2)) Enil ::: t2 ::: Enil)
+  | add_case6 t1 n2 => (* t1, Eop (Ointconst n2) Enil *) 
+      addimm n2 t1
+  | add_case7 t1 n2 t2 => (* t1, Eop (Oaddimm n2) (t2:::Enil) *) 
+      addimm n2 (Eop Oadd (t1:::t2:::Enil))
   | add_default e1 e2 =>
       Eop Oadd (e1:::e2:::Enil)
   end.
 
+
 (** ** Integer and pointer subtraction *)
 
-(*
-Definition sub (e1: expr) (e2: expr) :=
+(** Original definition:
+<<
+Nondetfunction sub (e1: expr) (e2: expr) :=
   match e1, e2 with
-  | t1, Eop (Ointconst n2) Enil => addimm (Int.neg n2) t1
-  | Eop (Oaddimm n1) (t1:::Enil), Eop (Oaddimm n2) (t2:::Enil) => addimm 
-(intsub n1 n2) (Eop Osub (t1:::t2:::Enil))
-  | Eop (Oaddimm n1) (t1:::Enil), t2 => addimm n1 (Eop Osub (t1:::t2:::Rni
-l))
-  | t1, Eop (Oaddimm n2) (t2:::Enil) => addimm (Int.neg n2) (Eop Osub (t1:::
-:t2:::Enil))
-  | _, _ => Eop Osub (e1:::e2:::Enil)
+  | t1, Eop (Ointconst n2) Enil =>
+      addimm (Int.neg n2) t1
+  | Eop (Oaddimm n1) (t1:::Enil), Eop (Oaddimm n2) (t2:::Enil) =>
+      addimm (Int.sub n1 n2) (Eop Osub (t1:::t2:::Enil))
+  | Eop (Oaddimm n1) (t1:::Enil), t2 =>
+      addimm n1 (Eop Osub (t1:::t2:::Enil))
+  | t1, Eop (Oaddimm n2) (t2:::Enil) =>
+      addimm (Int.neg n2) (Eop Osub (t1:::t2:::Enil))
+  | _, _ =>
+      Eop Osub (e1:::e2:::Enil)
   end.
+>>
 *)
 
 Inductive sub_cases: forall (e1: expr) (e2: expr), Type :=
-  | sub_case1:
-      forall (t1: expr) (n2: int),
-      sub_cases (t1) (Eop (Ointconst n2) Enil)
-  | sub_case2:
-      forall (n1: int) (t1: expr) (n2: int) (t2: expr),
-      sub_cases (Eop (Oaddimm n1) (t1:::Enil)) (Eop (Oaddimm n2) (t2:::Enil))
-  | sub_case3:
-      forall (n1: int) (t1: expr) (t2: expr),
-      sub_cases (Eop (Oaddimm n1) (t1:::Enil)) (t2)
-  | sub_case4:
-      forall (t1: expr) (n2: int) (t2: expr),
-      sub_cases (t1) (Eop (Oaddimm n2) (t2:::Enil))
-  | sub_default:
-      forall (e1: expr) (e2: expr),
-      sub_cases e1 e2.
-
-Definition sub_match_aux (e1: expr) (e2: expr) :=
-  match e1 as z1 return sub_cases z1 e2 with
-  | Eop (Oaddimm n1) (t1:::Enil) =>
-      sub_case3 n1 t1 e2
-  | e1 =>
-      sub_default e1 e2
-  end.
+  | sub_case1: forall t1 n2, sub_cases (t1) (Eop (Ointconst n2) Enil)
+  | sub_case2: forall n1 t1 n2 t2, sub_cases (Eop (Oaddimm n1) (t1:::Enil)) (Eop (Oaddimm n2) (t2:::Enil))
+  | sub_case3: forall n1 t1 t2, sub_cases (Eop (Oaddimm n1) (t1:::Enil)) (t2)
+  | sub_case4: forall t1 n2 t2, sub_cases (t1) (Eop (Oaddimm n2) (t2:::Enil))
+  | sub_default: forall (e1: expr) (e2: expr), sub_cases e1 e2.
 
 Definition sub_match (e1: expr) (e2: expr) :=
-  match e2 as z2, e1 as z1 return sub_cases z1 z2 with
-  | Eop (Ointconst n2) Enil, t1 =>
-      sub_case1 t1 n2
-  | Eop (Oaddimm n2) (t2:::Enil), Eop (Oaddimm n1) (t1:::Enil) =>
-      sub_case2 n1 t1 n2 t2
-  | Eop (Oaddimm n2) (t2:::Enil), t1 =>
-      sub_case4 t1 n2 t2
-  | e2, e1 =>
-      sub_match_aux e1 e2
+  match e1 as zz1, e2 as zz2 return sub_cases zz1 zz2 with
+  | t1, Eop (Ointconst n2) Enil => sub_case1 t1 n2
+  | Eop (Oaddimm n1) (t1:::Enil), Eop (Oaddimm n2) (t2:::Enil) => sub_case2 n1 t1 n2 t2
+  | Eop (Oaddimm n1) (t1:::Enil), t2 => sub_case3 n1 t1 t2
+  | t1, Eop (Oaddimm n2) (t2:::Enil) => sub_case4 t1 n2 t2
+  | e1, e2 => sub_default e1 e2
   end.
 
 Definition sub (e1: expr) (e2: expr) :=
   match sub_match e1 e2 with
-  | sub_case1 t1 n2 =>
+  | sub_case1 t1 n2 => (* t1, Eop (Ointconst n2) Enil *) 
       addimm (Int.neg n2) t1
-  | sub_case2 n1 t1 n2 t2 =>
+  | sub_case2 n1 t1 n2 t2 => (* Eop (Oaddimm n1) (t1:::Enil), Eop (Oaddimm n2) (t2:::Enil) *) 
       addimm (Int.sub n1 n2) (Eop Osub (t1:::t2:::Enil))
-  | sub_case3 n1 t1 t2 =>
+  | sub_case3 n1 t1 t2 => (* Eop (Oaddimm n1) (t1:::Enil), t2 *) 
       addimm n1 (Eop Osub (t1:::t2:::Enil))
-  | sub_case4 t1 n2 t2 =>
+  | sub_case4 t1 n2 t2 => (* t1, Eop (Oaddimm n2) (t2:::Enil) *) 
       addimm (Int.neg n2) (Eop Osub (t1:::t2:::Enil))
   | sub_default e1 e2 =>
       Eop Osub (e1:::e2:::Enil)
   end.
 
+
+Definition negint (e: expr) := Eop (Osubimm Int.zero) (e ::: Enil).
+
 (** ** Rotates and immediate shifts *)
 
-(** Recognition of integers that are acceptable as immediate operands
-  to the [rlwim] PowerPC instruction.  These integers are of the form
-  [000011110000] or [111100001111], that is, a run of one bits
-  surrounded by zero bits, or conversely.  We recognize these integers by
-  running the following automaton on the bits.  The accepting states are
-  2, 3, 4, 5, and 6.
+(** Original definition:
 <<
-               0          1          0
-              / \        / \        / \
-              \ /        \ /        \ /
-        -0--> [1] --1--> [2] --0--> [3]
-       /     
-     [0]
-       \
-        -1--> [4] --0--> [5] --1--> [6]
-              / \        / \        / \
-              \ /        \ /        \ /
-               1          0          1
->>
-*)
-
-Inductive rlw_state: Type :=
-  | RLW_S0 : rlw_state
-  | RLW_S1 : rlw_state
-  | RLW_S2 : rlw_state
-  | RLW_S3 : rlw_state
-  | RLW_S4 : rlw_state
-  | RLW_S5 : rlw_state
-  | RLW_S6 : rlw_state
-  | RLW_Sbad : rlw_state.
-
-Definition rlw_transition (s: rlw_state) (b: bool) : rlw_state :=
-  match s, b with
-  | RLW_S0, false => RLW_S1
-  | RLW_S0, true  => RLW_S4
-  | RLW_S1, false => RLW_S1
-  | RLW_S1, true  => RLW_S2
-  | RLW_S2, false => RLW_S3
-  | RLW_S2, true  => RLW_S2
-  | RLW_S3, false => RLW_S3
-  | RLW_S3, true  => RLW_Sbad
-  | RLW_S4, false => RLW_S5
-  | RLW_S4, true  => RLW_S4
-  | RLW_S5, false => RLW_S5
-  | RLW_S5, true  => RLW_S6
-  | RLW_S6, false => RLW_Sbad
-  | RLW_S6, true  => RLW_S6
-  | RLW_Sbad, _ => RLW_Sbad
-  end.
-
-Definition rlw_accepting (s: rlw_state) : bool :=
-  match s with
-  | RLW_S0 => false
-  | RLW_S1 => false
-  | RLW_S2 => true
-  | RLW_S3 => true
-  | RLW_S4 => true
-  | RLW_S5 => true
-  | RLW_S6 => true
-  | RLW_Sbad => false
-  end.
-
-Fixpoint is_rlw_mask_rec (n: nat) (s: rlw_state) (x: Z) {struct n} : bool :=
-  match n with
-  | O =>
-      rlw_accepting s
-  | S m =>
-      let (b, y) := Int.Z_bin_decomp x in
-      is_rlw_mask_rec m (rlw_transition s b) y
-  end.
-
-Definition is_rlw_mask (x: int) : bool :=
-  is_rlw_mask_rec Int.wordsize RLW_S0 (Int.unsigned x).
-
-(*
-Definition rolm (e1: expr) :=
+Nondetfunction rolm (e1: expr) (amount2: int) (mask2: int) :=
   match e1 with
   | Eop (Ointconst n1) Enil =>
       Eop (Ointconst(Int.and (Int.rol n1 amount2) mask2)) Enil
   | Eop (Orolm amount1 mask1) (t1:::Enil) =>
-      let amount := Int.and (Int.add amount1 amount2) Ox1Fl in
-      let mask := Int.and (Int.rol mask1 amount2) mask2 in
-      if Int.is_rlw_mask mask
-      then Eop (Orolm amount mask) (t1:::Enil)
-      else Eop (Orolm amount2 mask2) (e1:::Enil)
-  | _ => Eop (Orolm amount2 mask2) (e1:::Enil)
-  end
+      Eop (Orolm (Int.modu (Int.add amount1 amount2) Int.iwordsize)
+                 (Int.and (Int.rol mask1 amount2) mask2))
+          (t1:::Enil)
+  | _ =>
+      Eop (Orolm amount2 mask2) (e1:::Enil)
+  end.
+>>
 *)
 
-Inductive rolm_cases: forall (e1: expr), Type :=
-  | rolm_case1:
-      forall (n1: int),
-      rolm_cases (Eop (Ointconst n1) Enil)
-  | rolm_case2:
-      forall (amount1: int) (mask1: int) (t1: expr),
-      rolm_cases (Eop (Orolm amount1 mask1) (t1:::Enil))
-  | rolm_default:
-      forall (e1: expr),
-      rolm_cases e1.
+Inductive rolm_cases: forall (e1: expr) , Type :=
+  | rolm_case1: forall n1, rolm_cases (Eop (Ointconst n1) Enil)
+  | rolm_case2: forall amount1 mask1 t1, rolm_cases (Eop (Orolm amount1 mask1) (t1:::Enil))
+  | rolm_default: forall (e1: expr) , rolm_cases e1.
 
-Definition rolm_match (e1: expr) :=
-  match e1 as z1 return rolm_cases z1 with
-  | Eop (Ointconst n1) Enil =>
-      rolm_case1 n1
-  | Eop (Orolm amount1 mask1) (t1:::Enil) =>
-      rolm_case2 amount1 mask1 t1
-  | e1 =>
-      rolm_default e1
+Definition rolm_match (e1: expr)  :=
+  match e1 as zz1 return rolm_cases zz1 with
+  | Eop (Ointconst n1) Enil => rolm_case1 n1
+  | Eop (Orolm amount1 mask1) (t1:::Enil) => rolm_case2 amount1 mask1 t1
+  | e1 => rolm_default e1
   end.
 
-Definition rolm (e1: expr) (amount2 mask2: int) :=
+Definition rolm (e1: expr) (amount2: int) (mask2: int) :=
   match rolm_match e1 with
-  | rolm_case1 n1 =>
+  | rolm_case1 n1 => (* Eop (Ointconst n1) Enil *) 
       Eop (Ointconst(Int.and (Int.rol n1 amount2) mask2)) Enil
-  | rolm_case2 amount1 mask1 t1 =>
-      let amount := Int.modu (Int.add amount1 amount2) Int.iwordsize in
-      let mask := Int.and (Int.rol mask1 amount2) mask2 in
-      if is_rlw_mask mask
-      then Eop (Orolm amount mask) (t1:::Enil)
-      else Eop (Orolm amount2 mask2) (e1:::Enil)
+  | rolm_case2 amount1 mask1 t1 => (* Eop (Orolm amount1 mask1) (t1:::Enil) *) 
+      Eop (Orolm (Int.modu (Int.add amount1 amount2) Int.iwordsize) (Int.and (Int.rol mask1 amount2) mask2)) (t1:::Enil)
   | rolm_default e1 =>
       Eop (Orolm amount2 mask2) (e1:::Enil)
   end.
+
 
 Definition shlimm (e1: expr) (n2: int) :=
   if Int.eq n2 Int.zero then
@@ -518,6 +336,12 @@ Definition shlimm (e1: expr) (n2: int) :=
     rolm e1 n2 (Int.shl Int.mone n2)
   else
     Eop Oshl (e1:::Eop (Ointconst n2) Enil:::Enil).
+
+Definition shrimm (e1: expr) (n2: int) :=
+  if Int.eq n2 Int.zero then
+    e1
+  else
+    Eop (Oshrimm n2) (e1:::Enil).
 
 Definition shruimm (e1: expr) (n2: int) :=
   if Int.eq n2 Int.zero then
@@ -541,116 +365,113 @@ Definition mulimm_base (n1: int) (e2: expr) :=
       Eop (Omulimm n1) (e2:::Enil)
   end.
 
-(*
-Definition mulimm (n1: int) (e2: expr) :=
-  if Int.eq n1 Int.zero then 
-    Elet e2 (Eop (Ointconst Int.zero) Enil)
-  else if Int.eq n1 Int.one then
-    e2
+(** Original definition:
+<<
+Nondetfunction mulimm (n1: int) (e2: expr) :=
+  if Int.eq n1 Int.zero then Eop (Ointconst Int.zero) Enil
+  else if Int.eq n1 Int.one then e2
   else match e2 with
-  | Eop (Ointconst n2) Enil => Eop (Ointconst(intmul n1 n2)) Enil
-  | Eop (Oaddimm n2) (t2:::Enil) => addimm (intmul n1 n2) (mulimm_base n1 t2)
+  | Eop (Ointconst n2) Enil => Eop (Ointconst(Int.mul n1 n2)) Enil
+  | Eop (Oaddimm n2) (t2:::Enil) => addimm (Int.mul n1 n2) (mulimm_base n1 t2)
   | _ => mulimm_base n1 e2
   end.
+>>
 *)
 
 Inductive mulimm_cases: forall (e2: expr), Type :=
-  | mulimm_case1:
-      forall (n2: int),
-      mulimm_cases (Eop (Ointconst n2) Enil)
-  | mulimm_case2:
-      forall (n2: int) (t2: expr),
-      mulimm_cases (Eop (Oaddimm n2) (t2:::Enil))
-  | mulimm_default:
-      forall (e2: expr),
-      mulimm_cases e2.
+  | mulimm_case1: forall n2, mulimm_cases (Eop (Ointconst n2) Enil)
+  | mulimm_case2: forall n2 t2, mulimm_cases (Eop (Oaddimm n2) (t2:::Enil))
+  | mulimm_default: forall (e2: expr), mulimm_cases e2.
 
 Definition mulimm_match (e2: expr) :=
-  match e2 as z1 return mulimm_cases z1 with
-  | Eop (Ointconst n2) Enil =>
-      mulimm_case1 n2
-  | Eop (Oaddimm n2) (t2:::Enil) =>
-      mulimm_case2 n2 t2
-  | e2 =>
-      mulimm_default e2
+  match e2 as zz1 return mulimm_cases zz1 with
+  | Eop (Ointconst n2) Enil => mulimm_case1 n2
+  | Eop (Oaddimm n2) (t2:::Enil) => mulimm_case2 n2 t2
+  | e2 => mulimm_default e2
   end.
 
 Definition mulimm (n1: int) (e2: expr) :=
-  if Int.eq n1 Int.zero then 
-    Elet e2 (Eop (Ointconst Int.zero) Enil)
-  else if Int.eq n1 Int.one then
-    e2
-  else match mulimm_match e2 with
-  | mulimm_case1 n2 =>
+ if Int.eq n1 Int.zero then Eop (Ointconst Int.zero) Enil else if Int.eq n1 Int.one then e2 else match mulimm_match e2 with
+  | mulimm_case1 n2 => (* Eop (Ointconst n2) Enil *) 
       Eop (Ointconst(Int.mul n1 n2)) Enil
-  | mulimm_case2 n2 t2 =>
+  | mulimm_case2 n2 t2 => (* Eop (Oaddimm n2) (t2:::Enil) *) 
       addimm (Int.mul n1 n2) (mulimm_base n1 t2)
   | mulimm_default e2 =>
       mulimm_base n1 e2
   end.
 
-(*
-Definition mul (e1: expr) (e2: expr) :=
+
+(** Original definition:
+<<
+Nondetfunction mul (e1: expr) (e2: expr) :=
   match e1, e2 with
   | Eop (Ointconst n1) Enil, t2 => mulimm n1 t2
   | t1, Eop (Ointconst n2) Enil => mulimm n2 t1
   | _, _ => Eop Omul (e1:::e2:::Enil)
   end.
+>>
 *)
 
 Inductive mul_cases: forall (e1: expr) (e2: expr), Type :=
-  | mul_case1:
-      forall (n1: int) (t2: expr),
-      mul_cases (Eop (Ointconst n1) Enil) (t2)
-  | mul_case2:
-      forall (t1: expr) (n2: int),
-      mul_cases (t1) (Eop (Ointconst n2) Enil)
-  | mul_default:
-      forall (e1: expr) (e2: expr),
-      mul_cases e1 e2.
-
-Definition mul_match_aux (e1: expr) (e2: expr) :=
-  match e2 as z2 return mul_cases e1 z2 with
-  | Eop (Ointconst n2) Enil =>
-      mul_case2 e1 n2
-  | e2 =>
-      mul_default e1 e2
-  end.
+  | mul_case1: forall n1 t2, mul_cases (Eop (Ointconst n1) Enil) (t2)
+  | mul_case2: forall t1 n2, mul_cases (t1) (Eop (Ointconst n2) Enil)
+  | mul_default: forall (e1: expr) (e2: expr), mul_cases e1 e2.
 
 Definition mul_match (e1: expr) (e2: expr) :=
-  match e1 as z1 return mul_cases z1 e2 with
-  | Eop (Ointconst n1) Enil =>
-      mul_case1 n1 e2
-  | e1 =>
-      mul_match_aux e1 e2
+  match e1 as zz1, e2 as zz2 return mul_cases zz1 zz2 with
+  | Eop (Ointconst n1) Enil, t2 => mul_case1 n1 t2
+  | t1, Eop (Ointconst n2) Enil => mul_case2 t1 n2
+  | e1, e2 => mul_default e1 e2
   end.
 
 Definition mul (e1: expr) (e2: expr) :=
   match mul_match e1 e2 with
-  | mul_case1 n1 t2 =>
+  | mul_case1 n1 t2 => (* Eop (Ointconst n1) Enil, t2 *) 
       mulimm n1 t2
-  | mul_case2 t1 n2 =>
+  | mul_case2 t1 n2 => (* t1, Eop (Ointconst n2) Enil *) 
       mulimm n2 t1
   | mul_default e1 e2 =>
       Eop Omul (e1:::e2:::Enil)
   end.
 
+
 (** ** Bitwise and, or, xor *)
 
-Definition andimm (n1: int) (e2: expr) :=
-  if is_rlw_mask n1
-  then rolm e2 Int.zero n1
-  else Eop (Oandimm n1) (e2:::Enil).
+Definition andimm (n1: int) (e2: expr) := rolm e2 Int.zero n1.
+
+(** Original definition:
+<<
+Nondetfunction and (e1: expr) (e2: expr) :=
+  match e1, e2 with
+  | Eop (Ointconst n1) Enil, t2 => andimm n1 t2
+  | t1, Eop (Ointconst n2) Enil => andimm n2 t1
+  | _, _ => Eop Oand (e1:::e2:::Enil)
+  end.
+>>
+*)
+
+Inductive and_cases: forall (e1: expr) (e2: expr), Type :=
+  | and_case1: forall n1 t2, and_cases (Eop (Ointconst n1) Enil) (t2)
+  | and_case2: forall t1 n2, and_cases (t1) (Eop (Ointconst n2) Enil)
+  | and_default: forall (e1: expr) (e2: expr), and_cases e1 e2.
+
+Definition and_match (e1: expr) (e2: expr) :=
+  match e1 as zz1, e2 as zz2 return and_cases zz1 zz2 with
+  | Eop (Ointconst n1) Enil, t2 => and_case1 n1 t2
+  | t1, Eop (Ointconst n2) Enil => and_case2 t1 n2
+  | e1, e2 => and_default e1 e2
+  end.
 
 Definition and (e1: expr) (e2: expr) :=
-  match mul_match e1 e2 with
-  | mul_case1 n1 t2 =>
+  match and_match e1 e2 with
+  | and_case1 n1 t2 => (* Eop (Ointconst n1) Enil, t2 *) 
       andimm n1 t2
-  | mul_case2 t1 n2 =>
+  | and_case2 t1 n2 => (* t1, Eop (Ointconst n2) Enil *) 
       andimm n2 t1
-  | mul_default e1 e2 =>
+  | and_default e1 e2 =>
       Eop Oand (e1:::e2:::Enil)
   end.
+
 
 Definition same_expr_pure (e1 e2: expr) :=
   match e1, e2 with
@@ -658,30 +479,46 @@ Definition same_expr_pure (e1 e2: expr) :=
   | _, _ => false
   end.
 
-Inductive or_cases: forall (e1: expr) (e2: expr), Type :=
-  | or_case1:
-      forall (amount1: int) (mask1: int) (t1: expr)
-             (amount2: int) (mask2: int) (t2: expr),
-      or_cases (Eop (Orolm amount1  mask1) (t1:::Enil)) 
-               (Eop (Orolm amount2 mask2) (t2:::Enil))
-  | or_default:
-      forall (e1: expr) (e2: expr),
-      or_cases e1 e2.
+(** Original definition:
+<<
+Nondetfunction orimm (n1: int) (e2: expr) :=
+  match e2 with
+  | Eop (Ointconst n2) Enil => Eop (Ointconst (Int.or n1 n2)) Enil
+  | Eop (Oorimm n2) (t2:::Enil) => Eop (Oorimm (Int.or n1 n2)) (t2:::Enil)
+  | _ => Eop (Oorimm n1) (e2:::Enil)
+  end.
+>>
+*)
 
-Definition or_match (e1: expr) (e2: expr) :=
-  match e1 as z1, e2 as z2 return or_cases z1 z2 with
-  | Eop (Orolm amount1  mask1) (t1:::Enil),
-    Eop (Orolm amount2 mask2) (t2:::Enil) =>
-      or_case1 amount1 mask1 t1 amount2 mask2 t2
-  | e1, e2 =>
-      or_default e1 e2
+Inductive orimm_cases: forall (e2: expr), Type :=
+  | orimm_case1: forall n2, orimm_cases (Eop (Ointconst n2) Enil)
+  | orimm_case2: forall n2 t2, orimm_cases (Eop (Oorimm n2) (t2:::Enil))
+  | orimm_default: forall (e2: expr), orimm_cases e2.
+
+Definition orimm_match (e2: expr) :=
+  match e2 as zz1 return orimm_cases zz1 with
+  | Eop (Ointconst n2) Enil => orimm_case1 n2
+  | Eop (Oorimm n2) (t2:::Enil) => orimm_case2 n2 t2
+  | e2 => orimm_default e2
   end.
 
-Definition or (e1: expr) (e2: expr) :=
-  match or_match e1 e2 with
-  | or_case1 amount1 mask1 t1 amount2 mask2 t2 =>
+Definition orimm (n1: int) (e2: expr) :=
+  match orimm_match e2 with
+  | orimm_case1 n2 => (* Eop (Ointconst n2) Enil *) 
+      Eop (Ointconst (Int.or n1 n2)) Enil
+  | orimm_case2 n2 t2 => (* Eop (Oorimm n2) (t2:::Enil) *) 
+      Eop (Oorimm (Int.or n1 n2)) (t2:::Enil)
+  | orimm_default e2 =>
+      Eop (Oorimm n1) (e2:::Enil)
+  end.
+
+
+(** Original definition:
+<<
+Nondetfunction or (e1: expr) (e2: expr) :=
+  match e1, e2 with
+  | Eop (Orolm amount1  mask1) (t1:::Enil), Eop (Orolm amount2 mask2) (t2:::Enil) =>
       if Int.eq amount1 amount2
-      && is_rlw_mask (Int.or mask1 mask2)
       && same_expr_pure t1 t2 then
         Eop (Orolm amount1 (Int.or mask1 mask2)) (t1:::Enil)
       else if Int.eq amount1 Int.zero
@@ -692,9 +529,107 @@ Definition or (e1: expr) (e2: expr) :=
         Eop (Oroli amount1 mask1) (t2:::t1:::Enil)
       else
         Eop Oor (e1:::e2:::Enil)
+  | Eop (Ointconst n1) Enil, t2 => orimm n1 t2
+  | t1, Eop (Ointconst n2) Enil => orimm n2 t1
+  | _, _ => Eop Oor (e1:::e2:::Enil)
+  end.
+>>
+*)
+
+Inductive or_cases: forall (e1: expr) (e2: expr), Type :=
+  | or_case1: forall amount1 mask1 t1 amount2 mask2 t2, or_cases (Eop (Orolm amount1 mask1) (t1:::Enil)) (Eop (Orolm amount2 mask2) (t2:::Enil))
+  | or_case2: forall n1 t2, or_cases (Eop (Ointconst n1) Enil) (t2)
+  | or_case3: forall t1 n2, or_cases (t1) (Eop (Ointconst n2) Enil)
+  | or_default: forall (e1: expr) (e2: expr), or_cases e1 e2.
+
+Definition or_match (e1: expr) (e2: expr) :=
+  match e1 as zz1, e2 as zz2 return or_cases zz1 zz2 with
+  | Eop (Orolm amount1 mask1) (t1:::Enil), Eop (Orolm amount2 mask2) (t2:::Enil) => or_case1 amount1 mask1 t1 amount2 mask2 t2
+  | Eop (Ointconst n1) Enil, t2 => or_case2 n1 t2
+  | t1, Eop (Ointconst n2) Enil => or_case3 t1 n2
+  | e1, e2 => or_default e1 e2
+  end.
+
+Definition or (e1: expr) (e2: expr) :=
+  match or_match e1 e2 with
+  | or_case1 amount1 mask1 t1 amount2 mask2 t2 => (* Eop (Orolm amount1 mask1) (t1:::Enil), Eop (Orolm amount2 mask2) (t2:::Enil) *) 
+      if Int.eq amount1 amount2 && same_expr_pure t1 t2 then Eop (Orolm amount1 (Int.or mask1 mask2)) (t1:::Enil) else if Int.eq amount1 Int.zero && Int.eq mask1 (Int.not mask2) then Eop (Oroli amount2 mask2) (t1:::t2:::Enil) else if Int.eq amount2 Int.zero && Int.eq mask2 (Int.not mask1) then Eop (Oroli amount1 mask1) (t2:::t1:::Enil) else Eop Oor (e1:::e2:::Enil)
+  | or_case2 n1 t2 => (* Eop (Ointconst n1) Enil, t2 *) 
+      orimm n1 t2
+  | or_case3 t1 n2 => (* t1, Eop (Ointconst n2) Enil *) 
+      orimm n2 t1
   | or_default e1 e2 =>
       Eop Oor (e1:::e2:::Enil)
   end.
+
+
+(** Original definition:
+<<
+Nondetfunction xorimm (n1: int) (e2: expr) :=
+  match e2 with
+  | Eop (Ointconst n2) Enil => Eop (Ointconst (Int.xor n1 n2)) Enil
+  | Eop (Oxorimm n2) (t2:::Enil) => Eop (Oxorimm (Int.xor n1 n2)) (t2:::Enil)
+  | _ => Eop (Oxorimm n1) (e2:::Enil)
+  end.
+>>
+*)
+
+Inductive xorimm_cases: forall (e2: expr), Type :=
+  | xorimm_case1: forall n2, xorimm_cases (Eop (Ointconst n2) Enil)
+  | xorimm_case2: forall n2 t2, xorimm_cases (Eop (Oxorimm n2) (t2:::Enil))
+  | xorimm_default: forall (e2: expr), xorimm_cases e2.
+
+Definition xorimm_match (e2: expr) :=
+  match e2 as zz1 return xorimm_cases zz1 with
+  | Eop (Ointconst n2) Enil => xorimm_case1 n2
+  | Eop (Oxorimm n2) (t2:::Enil) => xorimm_case2 n2 t2
+  | e2 => xorimm_default e2
+  end.
+
+Definition xorimm (n1: int) (e2: expr) :=
+  match xorimm_match e2 with
+  | xorimm_case1 n2 => (* Eop (Ointconst n2) Enil *) 
+      Eop (Ointconst (Int.xor n1 n2)) Enil
+  | xorimm_case2 n2 t2 => (* Eop (Oxorimm n2) (t2:::Enil) *) 
+      Eop (Oxorimm (Int.xor n1 n2)) (t2:::Enil)
+  | xorimm_default e2 =>
+      Eop (Oxorimm n1) (e2:::Enil)
+  end.
+
+
+(** Original definition:
+<<
+Nondetfunction xor (e1: expr) (e2: expr) :=
+  match e1, e2 with
+  | Eop (Ointconst n1) Enil, t2 => xorimm n1 t2
+  | t1, Eop (Ointconst n2) Enil => xorimm n2 t1
+  | _, _ => Eop Oxor (e1:::e2:::Enil)
+  end.
+>>
+*)
+
+Inductive xor_cases: forall (e1: expr) (e2: expr), Type :=
+  | xor_case1: forall n1 t2, xor_cases (Eop (Ointconst n1) Enil) (t2)
+  | xor_case2: forall t1 n2, xor_cases (t1) (Eop (Ointconst n2) Enil)
+  | xor_default: forall (e1: expr) (e2: expr), xor_cases e1 e2.
+
+Definition xor_match (e1: expr) (e2: expr) :=
+  match e1 as zz1, e2 as zz2 return xor_cases zz1 zz2 with
+  | Eop (Ointconst n1) Enil, t2 => xor_case1 n1 t2
+  | t1, Eop (Ointconst n2) Enil => xor_case2 t1 n2
+  | e1, e2 => xor_default e1 e2
+  end.
+
+Definition xor (e1: expr) (e2: expr) :=
+  match xor_match e1 e2 with
+  | xor_case1 n1 t2 => (* Eop (Ointconst n1) Enil, t2 *) 
+      xorimm n1 t2
+  | xor_case2 t1 n2 => (* t1, Eop (Ointconst n2) Enil *) 
+      xorimm n2 t1
+  | xor_default e1 e2 =>
+      Eop Oxor (e1:::e2:::Enil)
+  end.
+
 
 (** ** Integer division and modulus *)
 
@@ -711,209 +646,325 @@ Definition mod_aux (divop: operation) (e1 e2: expr) :=
 
 Definition mods := mod_aux Odiv.
 
+Definition divuimm (e: expr) (n: int) :=
+  match Int.is_power2 n with
+  | Some l => shruimm e l
+  | None   => Eop Odivu (e ::: Eop (Ointconst n) Enil ::: Enil)
+  end.
+
+(** Original definition:
+<<
+Nondetfunction divu (e1: expr) (e2: expr) :=
+  match e2 with
+  | Eop (Ointconst n2) Enil => divuimm e1 n2
+  | _ => Eop Odivu (e1:::e2:::Enil)
+  end.
+>>
+*)
+
 Inductive divu_cases: forall (e2: expr), Type :=
-  | divu_case1:
-      forall (n2: int),
-      divu_cases (Eop (Ointconst n2) Enil)
-  | divu_default:
-      forall (e2: expr),
-      divu_cases e2.
+  | divu_case1: forall n2, divu_cases (Eop (Ointconst n2) Enil)
+  | divu_default: forall (e2: expr), divu_cases e2.
 
 Definition divu_match (e2: expr) :=
-  match e2 as z1 return divu_cases z1 with
-  | Eop (Ointconst n2) Enil =>
-      divu_case1 n2
-  | e2 =>
-      divu_default e2
+  match e2 as zz1 return divu_cases zz1 with
+  | Eop (Ointconst n2) Enil => divu_case1 n2
+  | e2 => divu_default e2
   end.
 
 Definition divu (e1: expr) (e2: expr) :=
   match divu_match e2 with
-  | divu_case1 n2 =>
-      match Int.is_power2 n2 with
-      | Some l2 => shruimm e1 l2
-      | None    => Eop Odivu (e1:::e2:::Enil)
-      end
+  | divu_case1 n2 => (* Eop (Ointconst n2) Enil *) 
+      divuimm e1 n2
   | divu_default e2 =>
       Eop Odivu (e1:::e2:::Enil)
   end.
 
+
+Definition moduimm (e: expr) (n: int) :=
+  match Int.is_power2 n with
+  | Some l => andimm (Int.sub n Int.one) e
+  | None   => mod_aux Odivu e (Eop (Ointconst n) Enil)
+  end.
+
+(** Original definition:
+<<
+Nondetfunction modu (e1: expr) (e2: expr) :=
+  match e2 with
+  | Eop (Ointconst n2) Enil => moduimm e1 n2
+  | _ => mod_aux Odivu e1 e2
+  end.
+>>
+*)
+
+Inductive modu_cases: forall (e2: expr), Type :=
+  | modu_case1: forall n2, modu_cases (Eop (Ointconst n2) Enil)
+  | modu_default: forall (e2: expr), modu_cases e2.
+
+Definition modu_match (e2: expr) :=
+  match e2 as zz1 return modu_cases zz1 with
+  | Eop (Ointconst n2) Enil => modu_case1 n2
+  | e2 => modu_default e2
+  end.
+
 Definition modu (e1: expr) (e2: expr) :=
-  match divu_match e2 with
-  | divu_case1 n2 =>
-      match Int.is_power2 n2 with
-      | Some l2 => andimm (Int.sub n2 Int.one) e1
-      | None    => mod_aux Odivu e1 e2
-      end
-  | divu_default e2 =>
+  match modu_match e2 with
+  | modu_case1 n2 => (* Eop (Ointconst n2) Enil *) 
+      moduimm e1 n2
+  | modu_default e2 =>
       mod_aux Odivu e1 e2
   end.
 
+
 (** ** General shifts *)
 
-Inductive shift_cases: forall (e1: expr), Type :=
-  | shift_case1:
-      forall (n2: int),
-      shift_cases (Eop (Ointconst n2) Enil)
-  | shift_default:
-      forall (e1: expr),
-      shift_cases e1.
+(** Original definition:
+<<
+Nondetfunction shl (e1: expr) (e2: expr) :=
+  match e2 with
+  | Eop (Ointconst n2) Enil => shlimm e1 n2
+  | _ => Eop Oshl (e1:::e2:::Enil)
+  end.
+>>
+*)
 
-Definition shift_match (e1: expr) :=
-  match e1 as z1 return shift_cases z1 with
-  | Eop (Ointconst n2) Enil =>
-      shift_case1 n2
-  | e1 =>
-      shift_default e1
+Inductive shl_cases: forall (e2: expr), Type :=
+  | shl_case1: forall n2, shl_cases (Eop (Ointconst n2) Enil)
+  | shl_default: forall (e2: expr), shl_cases e2.
+
+Definition shl_match (e2: expr) :=
+  match e2 as zz1 return shl_cases zz1 with
+  | Eop (Ointconst n2) Enil => shl_case1 n2
+  | e2 => shl_default e2
   end.
 
 Definition shl (e1: expr) (e2: expr) :=
-  match shift_match e2 with
-  | shift_case1 n2 =>
+  match shl_match e2 with
+  | shl_case1 n2 => (* Eop (Ointconst n2) Enil *) 
       shlimm e1 n2
-  | shift_default e2 =>
+  | shl_default e2 =>
       Eop Oshl (e1:::e2:::Enil)
   end.
 
+
+(** Original definition:
+<<
+Nondetfunction shr (e1: expr) (e2: expr) :=
+  match e2 with
+  | Eop (Ointconst n2) Enil => shrimm e1 n2
+  | _ => Eop Oshr (e1:::e2:::Enil)
+  end.
+>>
+*)
+
+Inductive shr_cases: forall (e2: expr), Type :=
+  | shr_case1: forall n2, shr_cases (Eop (Ointconst n2) Enil)
+  | shr_default: forall (e2: expr), shr_cases e2.
+
+Definition shr_match (e2: expr) :=
+  match e2 as zz1 return shr_cases zz1 with
+  | Eop (Ointconst n2) Enil => shr_case1 n2
+  | e2 => shr_default e2
+  end.
+
+Definition shr (e1: expr) (e2: expr) :=
+  match shr_match e2 with
+  | shr_case1 n2 => (* Eop (Ointconst n2) Enil *) 
+      shrimm e1 n2
+  | shr_default e2 =>
+      Eop Oshr (e1:::e2:::Enil)
+  end.
+
+
+(** Original definition:
+<<
+Nondetfunction shru (e1: expr) (e2: expr) :=
+  match e2 with
+  | Eop (Ointconst n2) Enil => shruimm e1 n2
+  | _ => Eop Oshru (e1:::e2:::Enil)
+  end.
+>>
+*)
+
+Inductive shru_cases: forall (e2: expr), Type :=
+  | shru_case1: forall n2, shru_cases (Eop (Ointconst n2) Enil)
+  | shru_default: forall (e2: expr), shru_cases e2.
+
+Definition shru_match (e2: expr) :=
+  match e2 as zz1 return shru_cases zz1 with
+  | Eop (Ointconst n2) Enil => shru_case1 n2
+  | e2 => shru_default e2
+  end.
+
 Definition shru (e1: expr) (e2: expr) :=
-  match shift_match e2 with
-  | shift_case1 n2 =>
+  match shru_match e2 with
+  | shru_case1 n2 => (* Eop (Ointconst n2) Enil *) 
       shruimm e1 n2
-  | shift_default e2 =>
+  | shru_default e2 =>
       Eop Oshru (e1:::e2:::Enil)
   end.
 
+
 (** ** Floating-point arithmetic *)
+
+Definition negf (e: expr) :=  Eop Onegf (e ::: Enil).
+Definition absf (e: expr) :=  Eop Oabsf (e ::: Enil).
 
 Parameter use_fused_mul : unit -> bool.
 
-(*
-Definition addf (e1: expr) (e2: expr) :=
+(** Original definition:
+<<
+Nondetfunction addf (e1: expr) (e2: expr) :=
+  if negb(use_fused_mul tt) then Eop Oaddf (e1:::e2:::Enil) else 
   match e1, e2 with
   | Eop Omulf (t1:::t2:::Enil), t3 => Eop Omuladdf (t1:::t2:::t3:::Enil)
-  | t1, Eop Omulf (t2:::t3:::Enil) => Elet t1 (Eop Omuladdf (t2:::t3:::Rvar 0:::Enil))
+  | t1, Eop Omulf (t2:::t3:::Enil) => Eop Omuladdf (t2:::t3:::t1:::Enil)
   | _, _ => Eop Oaddf (e1:::e2:::Enil)
   end.
+>>
 *)
 
 Inductive addf_cases: forall (e1: expr) (e2: expr), Type :=
-  | addf_case1:
-      forall (t1: expr) (t2: expr) (t3: expr),
-      addf_cases (Eop Omulf (t1:::t2:::Enil)) (t3)
-  | addf_case2:
-      forall (t1: expr) (t2: expr) (t3: expr),
-      addf_cases (t1) (Eop Omulf (t2:::t3:::Enil))
-  | addf_default:
-      forall (e1: expr) (e2: expr),
-      addf_cases e1 e2.
-
-Definition addf_match_aux (e1: expr) (e2: expr) :=
-  match e2 as z2 return addf_cases e1 z2 with
-  | Eop Omulf (t2:::t3:::Enil) =>
-      addf_case2 e1 t2 t3
-  | e2 =>
-      addf_default e1 e2
-  end.
+  | addf_case1: forall t1 t2 t3, addf_cases (Eop Omulf (t1:::t2:::Enil)) (t3)
+  | addf_case2: forall t1 t2 t3, addf_cases (t1) (Eop Omulf (t2:::t3:::Enil))
+  | addf_default: forall (e1: expr) (e2: expr), addf_cases e1 e2.
 
 Definition addf_match (e1: expr) (e2: expr) :=
-  match e1 as z1 return addf_cases z1 e2 with
-  | Eop Omulf (t1:::t2:::Enil) =>
-      addf_case1 t1 t2 e2
-  | e1 =>
-      addf_match_aux e1 e2
+  match e1 as zz1, e2 as zz2 return addf_cases zz1 zz2 with
+  | Eop Omulf (t1:::t2:::Enil), t3 => addf_case1 t1 t2 t3
+  | t1, Eop Omulf (t2:::t3:::Enil) => addf_case2 t1 t2 t3
+  | e1, e2 => addf_default e1 e2
   end.
 
 Definition addf (e1: expr) (e2: expr) :=
-  if use_fused_mul tt then
-    match addf_match e1 e2 with
-    | addf_case1 t1 t2 t3 =>
-        Eop Omuladdf (t1:::t2:::t3:::Enil)
-    | addf_case2 t1 t2 t3 =>
-        Eop Omuladdf (t2:::t3:::t1:::Enil)
-    | addf_default e1 e2 =>
-        Eop Oaddf (e1:::e2:::Enil)
-    end
-  else Eop Oaddf (e1:::e2:::Enil).
-
-(*
-Definition subf (e1: expr) (e2: expr) :=
-  match e1, e2 with
-  | Eop Omulfloat (t1:::t2:::Enil), t3 => Eop Omulsubf (t1:::t2:::t3:::Enil)
-  | _, _ => Eop Osubf (e1:::e2:::Enil)
+ if negb(use_fused_mul tt) then Eop Oaddf (e1:::e2:::Enil) else match addf_match e1 e2 with
+  | addf_case1 t1 t2 t3 => (* Eop Omulf (t1:::t2:::Enil), t3 *) 
+      Eop Omuladdf (t1:::t2:::t3:::Enil)
+  | addf_case2 t1 t2 t3 => (* t1, Eop Omulf (t2:::t3:::Enil) *) 
+      Eop Omuladdf (t2:::t3:::t1:::Enil)
+  | addf_default e1 e2 =>
+      Eop Oaddf (e1:::e2:::Enil)
   end.
+
+
+(** Original definition:
+<<
+Nondetfunction subf (e1: expr) (e2: expr) :=
+  if negb(use_fused_mul tt) then Eop Osubf (e1:::e2:::Enil) else 
+  match e1 with
+  | Eop Omulf (t1:::t2:::Enil) => Eop Omulsubf (t1:::t2:::e2:::Enil)
+  | _ => Eop Osubf (e1:::e2:::Enil)
+  end.
+>>
 *)
 
-Inductive subf_cases: forall (e1: expr) (e2: expr), Type :=
-  | subf_case1:
-      forall (t1: expr) (t2: expr) (t3: expr),
-      subf_cases (Eop Omulf (t1:::t2:::Enil)) (t3)
-  | subf_default:
-      forall (e1: expr) (e2: expr),
-      subf_cases e1 e2.
+Inductive subf_cases: forall (e1: expr) , Type :=
+  | subf_case1: forall t1 t2, subf_cases (Eop Omulf (t1:::t2:::Enil))
+  | subf_default: forall (e1: expr) , subf_cases e1.
 
-Definition subf_match (e1: expr) (e2: expr) :=
-  match e1 as z1 return subf_cases z1 e2 with
-  | Eop Omulf (t1:::t2:::Enil) =>
-      subf_case1 t1 t2 e2
-  | e1 =>
-      subf_default e1 e2
+Definition subf_match (e1: expr)  :=
+  match e1 as zz1 return subf_cases zz1 with
+  | Eop Omulf (t1:::t2:::Enil) => subf_case1 t1 t2
+  | e1 => subf_default e1
   end.
 
 Definition subf (e1: expr) (e2: expr) :=
-  if use_fused_mul tt then
-    match subf_match e1 e2 with
-    | subf_case1 t1 t2 t3 =>
-        Eop Omulsubf (t1:::t2:::t3:::Enil)
-    | subf_default e1 e2 =>
-        Eop Osubf (e1:::e2:::Enil)
-    end
-  else Eop Osubf (e1:::e2:::Enil).
+ if negb(use_fused_mul tt) then Eop Osubf (e1:::e2:::Enil) else match subf_match e1 with
+  | subf_case1 t1 t2 => (* Eop Omulf (t1:::t2:::Enil) *) 
+      Eop Omulsubf (t1:::t2:::e2:::Enil)
+  | subf_default e1 =>
+      Eop Osubf (e1:::e2:::Enil)
+  end.
+
+
+Definition mulf (e1 e2: expr) :=  Eop Omulf (e1 ::: e2 ::: Enil).
+Definition divf (e1 e2: expr) :=  Eop Odivf (e1 ::: e2 ::: Enil).
 
 (** ** Comparisons *)
 
+(** Original definition:
+<<
+Nondetfunction comp (c: comparison) (e1: expr) (e2: expr) :=
+  match e1, e2 with
+  | Eop (Ointconst n1) Enil, t2 =>
+      Eop (Ocmp (Ccompimm (swap_comparison c) n1)) (t2 ::: Enil)
+  | t1, Eop (Ointconst n2) Enil =>
+      Eop (Ocmp (Ccompimm c n2)) (t1 ::: Enil)
+  | _, _ =>
+      Eop (Ocmp (Ccomp c)) (e1 ::: e2 ::: Enil)
+  end.
+>>
+*)
+
 Inductive comp_cases: forall (e1: expr) (e2: expr), Type :=
-  | comp_case1:
-      forall n1 t2,
-      comp_cases (Eop (Ointconst n1) Enil) (t2)
-  | comp_case2:
-      forall t1 n2,
-      comp_cases (t1) (Eop (Ointconst n2) Enil)
-  | comp_default:
-      forall (e1: expr) (e2: expr),
-      comp_cases e1 e2.
+  | comp_case1: forall n1 t2, comp_cases (Eop (Ointconst n1) Enil) (t2)
+  | comp_case2: forall t1 n2, comp_cases (t1) (Eop (Ointconst n2) Enil)
+  | comp_default: forall (e1: expr) (e2: expr), comp_cases e1 e2.
 
 Definition comp_match (e1: expr) (e2: expr) :=
-  match e1 as z1, e2 as z2 return comp_cases z1 z2 with
-  | Eop (Ointconst n1) Enil, t2 =>
-      comp_case1 n1 t2
-  | t1, Eop (Ointconst n2) Enil =>
-      comp_case2 t1 n2
-  | e1, e2 =>
-      comp_default e1 e2
+  match e1 as zz1, e2 as zz2 return comp_cases zz1 zz2 with
+  | Eop (Ointconst n1) Enil, t2 => comp_case1 n1 t2
+  | t1, Eop (Ointconst n2) Enil => comp_case2 t1 n2
+  | e1, e2 => comp_default e1 e2
   end.
 
 Definition comp (c: comparison) (e1: expr) (e2: expr) :=
   match comp_match e1 e2 with
-  | comp_case1 n1 t2 =>
+  | comp_case1 n1 t2 => (* Eop (Ointconst n1) Enil, t2 *) 
       Eop (Ocmp (Ccompimm (swap_comparison c) n1)) (t2 ::: Enil)
-  | comp_case2 t1 n2 =>
+  | comp_case2 t1 n2 => (* t1, Eop (Ointconst n2) Enil *) 
       Eop (Ocmp (Ccompimm c n2)) (t1 ::: Enil)
   | comp_default e1 e2 =>
       Eop (Ocmp (Ccomp c)) (e1 ::: e2 ::: Enil)
   end.
 
-Definition compu (c: comparison) (e1: expr) (e2: expr) :=
-  match comp_match e1 e2 with
-  | comp_case1 n1 t2 =>
+
+(** Original definition:
+<<
+Nondetfunction compu (c: comparison) (e1: expr) (e2: expr) :=
+  match e1, e2 with
+  | Eop (Ointconst n1) Enil, t2 =>
       Eop (Ocmp (Ccompuimm (swap_comparison c) n1)) (t2 ::: Enil)
-  | comp_case2 t1 n2 =>
+  | t1, Eop (Ointconst n2) Enil =>
       Eop (Ocmp (Ccompuimm c n2)) (t1 ::: Enil)
-  | comp_default e1 e2 =>
+  | _, _ =>
+      Eop (Ocmp (Ccompu c)) (e1 ::: e2 ::: Enil)
+  end.
+>>
+*)
+
+Inductive compu_cases: forall (e1: expr) (e2: expr), Type :=
+  | compu_case1: forall n1 t2, compu_cases (Eop (Ointconst n1) Enil) (t2)
+  | compu_case2: forall t1 n2, compu_cases (t1) (Eop (Ointconst n2) Enil)
+  | compu_default: forall (e1: expr) (e2: expr), compu_cases e1 e2.
+
+Definition compu_match (e1: expr) (e2: expr) :=
+  match e1 as zz1, e2 as zz2 return compu_cases zz1 zz2 with
+  | Eop (Ointconst n1) Enil, t2 => compu_case1 n1 t2
+  | t1, Eop (Ointconst n2) Enil => compu_case2 t1 n2
+  | e1, e2 => compu_default e1 e2
+  end.
+
+Definition compu (c: comparison) (e1: expr) (e2: expr) :=
+  match compu_match e1 e2 with
+  | compu_case1 n1 t2 => (* Eop (Ointconst n1) Enil, t2 *) 
+      Eop (Ocmp (Ccompuimm (swap_comparison c) n1)) (t2 ::: Enil)
+  | compu_case2 t1 n2 => (* t1, Eop (Ointconst n2) Enil *) 
+      Eop (Ocmp (Ccompuimm c n2)) (t1 ::: Enil)
+  | compu_default e1 e2 =>
       Eop (Ocmp (Ccompu c)) (e1 ::: e2 ::: Enil)
   end.
 
+
 Definition compf (c: comparison) (e1: expr) (e2: expr) :=
   Eop (Ocmp (Ccompf c)) (e1 ::: e2 ::: Enil).
+
+(** ** Integer conversions *)
+
+Definition cast8unsigned (e: expr) := andimm (Int.repr 255) e.
+Definition cast8signed (e: expr) := Eop Ocast8signed (e ::: Enil).
+Definition cast16unsigned (e: expr) := andimm (Int.repr 65535) e.
+Definition cast16signed (e: expr) := Eop Ocast16signed (e ::: Enil).
 
 (** ** Floating-point conversions *)
 
@@ -935,84 +986,55 @@ Definition floatofint (e: expr) :=
                            ::: addimm Float.ox8000_0000 e ::: Enil))
        (Eop (Ofloatconst (Float.from_words Float.ox4330_0000 Float.ox8000_0000)) Enil).
 
-(** ** Other operators, not optimized. *)
-
-Definition cast8unsigned (e: expr) := Eop Ocast8unsigned (e ::: Enil).
-Definition cast8signed (e: expr) := Eop Ocast8signed (e ::: Enil).
-Definition cast16unsigned (e: expr) := Eop Ocast16unsigned (e ::: Enil).
-Definition cast16signed (e: expr) := Eop Ocast16signed (e ::: Enil).
 Definition singleoffloat (e: expr) := Eop Osingleoffloat (e ::: Enil).
-Definition negint (e: expr) := Eop (Osubimm Int.zero) (e ::: Enil).
-Definition negf (e: expr) :=  Eop Onegf (e ::: Enil).
-Definition absf (e: expr) :=  Eop Oabsf (e ::: Enil).
-Definition xor (e1 e2: expr) :=  Eop Oxor (e1 ::: e2 ::: Enil).
-Definition shr (e1 e2: expr) :=  Eop Oshr (e1 ::: e2 ::: Enil).
-Definition mulf (e1 e2: expr) :=  Eop Omulf (e1 ::: e2 ::: Enil).
-Definition divf (e1 e2: expr) :=  Eop Odivf (e1 ::: e2 ::: Enil).
 
 (** ** Recognition of addressing modes for load and store operations *)
 
-(*
-Definition addressing (e: expr) :=
+(** Original definition:
+<<
+Nondetfunction addressing (chunk: memory_chunk) (e: expr) :=
   match e with
   | Eop (Oaddrsymbol s n) Enil => (Aglobal s n, Enil)
   | Eop (Oaddrstack n) Enil => (Ainstack n, Enil)
-  | Eop Oadd (Eop (Oaddrsymbol s n) Enil) e2 => (Abased(s, n), e2:::Enil)
+  | Eop Oadd (Eop (Oaddrsymbol s n) Enil ::: e2 ::: Enil) => (Abased s n, e2:::Enil)
   | Eop (Oaddimm n) (e1:::Enil) => (Aindexed n, e1:::Enil)
   | Eop Oadd (e1:::e2:::Enil) => (Aindexed2, e1:::e2:::Enil)
   | _ => (Aindexed Int.zero, e:::Enil)
   end.
+>>
 *)
 
 Inductive addressing_cases: forall (e: expr), Type :=
-  | addressing_case1:
-      forall (s: ident) (n: int),
-      addressing_cases (Eop (Oaddrsymbol s n) Enil)
-  | addressing_case2:
-      forall (n: int),
-      addressing_cases (Eop (Oaddrstack n) Enil)
-  | addressing_case3:
-      forall (s: ident) (n: int) (e2: expr),
-      addressing_cases
-        (Eop Oadd (Eop (Oaddrsymbol s n) Enil:::e2:::Enil))
-  | addressing_case4:
-      forall (n: int) (e1: expr),
-      addressing_cases (Eop (Oaddimm n) (e1:::Enil))
-  | addressing_case5:
-      forall (e1: expr) (e2: expr),
-      addressing_cases (Eop Oadd (e1:::e2:::Enil))
-  | addressing_default:
-      forall (e: expr),
-      addressing_cases e.
+  | addressing_case1: forall s n, addressing_cases (Eop (Oaddrsymbol s n) Enil)
+  | addressing_case2: forall n, addressing_cases (Eop (Oaddrstack n) Enil)
+  | addressing_case3: forall s n e2, addressing_cases (Eop Oadd (Eop (Oaddrsymbol s n) Enil ::: e2 ::: Enil))
+  | addressing_case4: forall n e1, addressing_cases (Eop (Oaddimm n) (e1:::Enil))
+  | addressing_case5: forall e1 e2, addressing_cases (Eop Oadd (e1:::e2:::Enil))
+  | addressing_default: forall (e: expr), addressing_cases e.
 
 Definition addressing_match (e: expr) :=
-  match e as z1 return addressing_cases z1 with
-  | Eop (Oaddrsymbol s n) Enil =>
-      addressing_case1 s n
-  | Eop (Oaddrstack n) Enil =>
-      addressing_case2 n
-  | Eop Oadd (Eop (Oaddrsymbol s n) Enil:::e2:::Enil) =>
-      addressing_case3 s n e2
-  | Eop (Oaddimm n) (e1:::Enil) =>
-      addressing_case4 n e1
-  | Eop Oadd (e1:::e2:::Enil) =>
-      addressing_case5 e1 e2
-  | e =>
-      addressing_default e
+  match e as zz1 return addressing_cases zz1 with
+  | Eop (Oaddrsymbol s n) Enil => addressing_case1 s n
+  | Eop (Oaddrstack n) Enil => addressing_case2 n
+  | Eop Oadd (Eop (Oaddrsymbol s n) Enil ::: e2 ::: Enil) => addressing_case3 s n e2
+  | Eop (Oaddimm n) (e1:::Enil) => addressing_case4 n e1
+  | Eop Oadd (e1:::e2:::Enil) => addressing_case5 e1 e2
+  | e => addressing_default e
   end.
 
 Definition addressing (chunk: memory_chunk) (e: expr) :=
   match addressing_match e with
-  | addressing_case1 s n =>
+  | addressing_case1 s n => (* Eop (Oaddrsymbol s n) Enil *) 
       (Aglobal s n, Enil)
-  | addressing_case2 n =>
+  | addressing_case2 n => (* Eop (Oaddrstack n) Enil *) 
       (Ainstack n, Enil)
-  | addressing_case3 s n e2 =>
+  | addressing_case3 s n e2 => (* Eop Oadd (Eop (Oaddrsymbol s n) Enil ::: e2 ::: Enil) *) 
       (Abased s n, e2:::Enil)
-  | addressing_case4 n e1 =>
+  | addressing_case4 n e1 => (* Eop (Oaddimm n) (e1:::Enil) *) 
       (Aindexed n, e1:::Enil)
-  | addressing_case5 e1 e2 =>
+  | addressing_case5 e1 e2 => (* Eop Oadd (e1:::e2:::Enil) *) 
       (Aindexed2, e1:::e2:::Enil)
   | addressing_default e =>
       (Aindexed Int.zero, e:::Enil)
   end.
+
